clang/spec.v
@@ -1,0 +1,94 @@
+(* Spec Monoid *)
+
+Require Import logic.
+From iris.base_logic Require Import gen_heap big_op.
+From iris.algebra Require Import gmap agree auth.
+From iris.base_logic.lib Require Import wsat fancy_updates.
+From iris.proofmode Require Import tactics.
+Set Default Proof Using "Type".
+Import uPred.
+
+Definition spec_state := gmap ident val. (* XXX: should be parameterized *)
+
+Definition spec_rel := spec_state → option val → spec_state → Prop.
+
+Inductive spec_code :=
+| SCrel (r: spec_rel)
+| SCdone (v: option val).
+
+Inductive spec_step : spec_code → spec_state → spec_code → spec_state → Prop :=
+| spec_step_rel:
+    ∀ (r: spec_rel) s retv s',
+      r s retv s' → spec_step (SCrel r) s (SCdone retv) s'.
+
+(* Naive equivalence *)
+Instance spec_code_equiv: Equiv spec_code := (=).
+
+Class specG Σ := SpecG {
+  specG_spstG :> gen_heapG ident val Σ;
+  specG_specG :> inG Σ (authR (optionUR (agreeR (discreteC (spec_code)))));
+  spec_gname : gname
+}.
+
+Notation "l S↦ v" :=
+  (@mapsto _ _ _ _ _ specG_spstG l 1%Qp v) (at level 20) : uPred_scope.
+
+Section rules.
+  Context `{specG Σ}.
+
+  Definition γ_sstate := @gen_heap_name _ _ _ _ _ specG_spstG.
+
+  Definition sstate (s: spec_state) := ([⋅ map] l ↦ v ∈ s, l S↦ v)%I.
+  Definition scode (c: spec_code) := own spec_gname (◯ (Some (to_agree (c: leibnizC spec_code)))).
+  
+  Definition spec_inv :=
+    (∃ c0 s0 c s,
+     own spec_gname (● (Some (to_agree (c : leibnizC spec_code)))) ∗
+     own γ_sstate (● to_gen_heap s) ∗ ⌜ spec_step c0 s0 c s⌝)%I.
+
+  Lemma spec_step_framing c c' sf s s':
+    gset_dom sf ⊥ gset_dom s → spec_step c s c' s' → spec_step c (sf ∪ s) c' (sf ∪ s').
+  Admitted.
+
+  Lemma spec_step_trans c c' c'' s s' s'':
+    spec_step c s c' s' → spec_step c' s' c'' s'' → spec_step c s c'' s''.
+  Admitted.
+
+  Lemma sstate_update s ss ss':
+    own γ_sstate (● to_gen_heap s) ∗
+    ([∗ map] l↦v ∈ ss, l S↦ v)
+    ⊢ (∃ s', own γ_sstate (● to_gen_heap s') ∗
+             ([∗ map] l↦v ∈ ss', l S↦ v) ∗
+             ⌜ ∃ sf, gset_dom sf ⊥ gset_dom ss ∧ s = sf ∪ ss ∧ s' = sf ∪ ss' ⌝).
+  Proof.
+  Admitted.
+
+  Lemma scode_update c1 c2 c3:
+    own spec_gname (● Some (to_agree c1)) ∗
+    own spec_gname (◯ Some (to_agree c2))
+    ⊢ own spec_gname (● Some (to_agree c3)) ∗
+      own spec_gname (◯ Some (to_agree c3)) ∗ ⌜ c1 = c2 ⌝.
+  Admitted.
+    
+  Lemma spec_update ss sc ss' sc':
+    spec_inv ∗ sstate ss ∗ scode sc ∗
+    ⌜ spec_step sc ss sc' ss' ⌝
+    ⊢ spec_inv ∗ sstate ss' ∗ scode sc'.
+  Proof.
+    iIntros "(Hinv & Hss & Hsc & %)".
+    iDestruct "Hinv" as (c0 s0 c s) "(HSC & HSS & %)".
+    rewrite /sstate /scode.
+    (* HSC Hsc and sc' are easy to prove *)
+    (* ss, s => ss' are hard, might need some framing properties *)
+    iDestruct (sstate_update s ss ss' with "[HSS Hss]") as (s') "(HSS' & Hss' & %)"; first iFrame.
+    iDestruct (scode_update _ _ sc' with "[HSC Hsc]") as "(HSC' & Hsc' & %)"; first iFrame.
+    iSplitL "HSS' HSC'".
+    { iExists c0, s0, sc', s'. iFrame.
+      destruct H2 as (sf & ? & ? & ?).
+      subst. iPureIntro.
+      assert (spec_step sc (sf ∪ ss) sc' (sf ∪ ss')) as ?; first by apply spec_step_framing.
+      eapply spec_step_trans=>//.
+    }
+    iFrame.
+  Qed.
+End rules.
